Launchbury/ArityEtaExpand.thy
@@ -1,0 +1,197 @@
+theory ArityEtaExpand
+imports ArityCorrectSestoft EtaExpansion
+begin
+
+locale ArityEtaExpand = CorrectArityAnalysisAheap +
+  fixes Aeta_expand_transform :: "Arity \<Rightarrow> exp \<Rightarrow> exp"
+begin
+
+  definition Aeta_expand :: "Arity \<Rightarrow> exp \<Rightarrow> exp" 
+    where "Aeta_expand a e = eta_expand (Rep_Arity a) e"
+  lemma Aeta_expand_0[simp]: "Aeta_expand 0 e = e"
+    unfolding Aeta_expand_def by (metis eta_expand.simps(1) zero_Arity.rep_eq)
+
+  lemma Aeta_expand_correct:
+    assumes "ae ` upds S \<subseteq> {up \<cdot> 0}"  
+    assumes "Astack ae S \<sqsubseteq> a"
+    shows "(\<Gamma>, Aeta_expand a e, S) \<Rightarrow>\<^sup>* (\<Gamma>, e, S)"
+  proof-
+    from assms(1)
+    have "arg_prefix S = Rep_Arity (Astack ae S)"
+      by (induction S arbitrary: a rule: arg_prefix.induct) (auto simp add: Arity.zero_Arity.rep_eq[symmetric])
+    also
+    from assms(2)
+    have "Rep_Arity a \<le> Rep_Arity (Astack ae S)" by (metis below_Arity.rep_eq)
+    finally
+    show ?thesis unfolding Aeta_expand_def by (rule eta_expansion_correct')
+  qed
+
+  lemma isLam_Aeta_expand: "isLam e \<Longrightarrow> isLam (Aeta_expand a e)"
+    unfolding Aeta_expand_def by (rule isLam_eta_expand)
+
+  fun Aeta_expand' :: "Arity\<^sub>\<bottom> \<Rightarrow> exp \<Rightarrow> exp" 
+  where "Aeta_expand' (Iup a) e = Aeta_expand a e"
+   |    "Aeta_expand' Ibottom e = e"
+
+  lemma [simp]: "Aeta_expand' (up\<cdot>a) e = Aeta_expand a e" unfolding up_def by (simp add: cont_Iup)
+
+  fun Aeta_expand_transform' :: "Arity\<^sub>\<bottom> \<Rightarrow> exp \<Rightarrow> exp" 
+  where "Aeta_expand_transform' (Iup a) e = Aeta_expand_transform a e"
+   |    "Aeta_expand_transform' Ibottom e = e"
+
+  lemma [simp]: "Aeta_expand_transform' (up\<cdot>a) e = Aeta_expand_transform a e" unfolding up_def by (simp add: cont_Iup)
+
+  fun Atransform :: "(AEnv \<times> Arity) \<Rightarrow> conf \<Rightarrow> conf"
+  where "Atransform (ae, a) (\<Gamma>, e, S) =
+    (map_ran (\<lambda> x e. Aeta_expand' (ae x) (Aeta_expand_transform' (ae x) e)) \<Gamma>, 
+     Aeta_expand_transform a e,
+     S)"
+
+  inductive consistent  where
+    [intro!]: "AE_consistent ae (\<Gamma>, e, S) \<Longrightarrow> Astack ae S \<sqsubseteq> a \<Longrightarrow> consistent (ae, a) (\<Gamma>, e, S)"
+  declare consistent.cases[elim!]
+
+  lemma [simp]:
+    "Aeta_expand_transform a (App e x) = App (Aeta_expand_transform (inc\<cdot>a) e) x"
+    "Aeta_expand_transform a (Lam [x]. e) = Lam [x].(Aeta_expand_transform (pred\<cdot>a) e)"
+    "Aeta_expand_transform a (e[x ::= z]) = (Aeta_expand_transform a e)[x ::= z]"
+    "Aeta_expand_transform a (Var x) = Var x"
+    "isLam (Aeta_expand_transform a e) \<longleftrightarrow> isLam e"
+    sorry
+
+  sublocale AbstractConforms step consistent.
+
+lemma foo:
+  fixes c c' R 
+  assumes "c \<Rightarrow> c'" and "consistent (ae,a) c"
+  shows "\<exists>ae' a'. consistent (ae',a') c' \<and> Atransform (ae,a) c \<Rightarrow>\<^sup>* Atransform (ae',a') c'"
+using assms
+proof(induction)
+case (app\<^sub>1 \<Gamma> e x S)
+  from app\<^sub>1 have "AE_consistent ae (\<Gamma>, e, Arg x # S)"  by (fastforce intro!: AE_consistentI simp add: Aexp_App join_below_iff)
+  moreover
+  have "Astack ae (Arg x # S) \<sqsubseteq> inc\<cdot>a" using app\<^sub>1 by (auto intro: monofun_cfun_arg)
+  ultimately
+  have "consistent (ae, inc\<cdot>a) (\<Gamma>, e, Arg x # S)" ..
+  moreover
+  have "Atransform (ae, a) (\<Gamma>, App e x, S) \<Rightarrow> Atransform (ae, inc\<cdot>a) (\<Gamma>, e, Arg x # S)" by simp rule
+  ultimately
+  show ?case by blast
+next
+case (app\<^sub>2 \<Gamma> y e x S)
+  hence "AE_consistent ae (\<Gamma>, e[y::=x], S)" 
+    by (fastforce intro!: AE_consistentI  below_trans[OF monofun_cfun_fun[OF Aexp_subst_App_Lam]] simp add: Aexp_App join_below_iff)
+  moreover
+  have "Astack ae S \<sqsubseteq> pred\<cdot>a" using app\<^sub>2 by (auto, metis monofun_cfun_arg pred_inc)
+  ultimately
+  have "consistent (ae, pred\<cdot>a) (\<Gamma>, e[y ::= x], S)" ..
+  moreover
+  have "Atransform (ae, a) (\<Gamma>, Lam [y]. e, Arg x # S) \<Rightarrow> Atransform (ae, pred \<cdot> a) (\<Gamma>, e[y::=x], S)" by simp rule
+  ultimately
+  show ?case by blast
+next
+case (var\<^sub>1 \<Gamma> x e S)
+  from var\<^sub>1 have "Aexp (Var x)\<cdot>(Astack ae S) \<sqsubseteq> ae" by auto
+  from below_trans[OF Aexp_Var fun_belowD[OF this] ]
+  have "up\<cdot>(Astack ae S) \<sqsubseteq> ae x".
+  then obtain u where "ae x = up\<cdot>u" and "Astack ae S \<sqsubseteq> u" by (cases "ae x") auto
+  moreover
+  hence "x \<in> edom ae" unfolding edom_def by auto
+  ultimately
+  have "AE_consistent ae (delete x \<Gamma>, e, Upd x # S)" using var\<^sub>1 by (fastforce intro!: AE_consistentI  simp add: join_below_iff)
+  moreover
+  have "Astack ae (Upd x # S) \<sqsubseteq> 0" by simp
+  ultimately
+  have "consistent (ae, 0) (delete x \<Gamma>, e, Upd x # S)" by blast
+  moreover
+  {
+  from var\<^sub>1 have "ae x = up\<cdot>0" by auto
+  with  `map_of \<Gamma> x = Some e`
+  have "map_of (map_ran (\<lambda>x e. Aeta_expand' (ae x) (Aeta_expand_transform' (ae x) e)) \<Gamma>) x = Some (Aeta_expand_transform 0 e)"
+    by (simp add: map_ran_conv)
+  with `\<not> isLam e`
+  have "Atransform (ae, a) (\<Gamma>, Var x, S) \<Rightarrow> Atransform (ae, 0) (delete x \<Gamma>, e, Upd x # S)"
+    by (auto simp add: map_ran_delete intro!: step.intros)
+  }
+  ultimately
+  show ?case by blast
+next 
+case (var\<^sub>2 \<Gamma> x e S)
+  from var\<^sub>2 have "ae ` upds S \<subseteq> {up \<cdot> 0}" by fastforce
+
+  from var\<^sub>2 have "Aexp (Var x)\<cdot>(Astack ae S) \<sqsubseteq> ae" by auto
+  from below_trans[OF Aexp_Var fun_belowD[OF this] ]
+  have "up\<cdot>(Astack ae S) \<sqsubseteq> ae x".
+  then obtain u where "ae x = up\<cdot>u" and "Astack ae S \<sqsubseteq> u" by (cases "ae x") auto
+
+  from this(2)
+  have "Aexp e\<cdot>(Astack ae S) \<sqsubseteq> Aexp e\<cdot>u" by (rule monofun_cfun_arg)
+  also have "\<dots> \<sqsubseteq> ae" using `ae x = up \<cdot> u` var\<^sub>2 by fastforce
+  finally have "Aexp e\<cdot>(Astack ae S) \<sqsubseteq> ae" by this simp
+  hence "AE_consistent ae ((x, e) # delete x \<Gamma>, e, S)"
+    using var\<^sub>2 by(fastforce intro!: AE_consistentI  simp add: join_below_iff split:if_splits)
+  moreover
+  have "Astack ae S \<sqsubseteq> u" by fact
+  ultimately
+  have "consistent (ae, u) ((x, e) # delete x \<Gamma>, e, S)" by auto
+  moreover
+  {
+  from `isLam e`
+  have "isLam (Aeta_expand_transform u e)" by simp
+  hence "isLam (Aeta_expand u (Aeta_expand_transform u e))" by (rule isLam_Aeta_expand)
+  moreover
+  from  `map_of \<Gamma> x = Some e`  `ae x = up \<cdot> u`
+  have "map_of (map_ran (\<lambda>x e. Aeta_expand' (ae x) (Aeta_expand_transform' (ae x) e)) \<Gamma>) x 
+    = Some (Aeta_expand u (Aeta_expand_transform u e))"
+    by (simp add: map_ran_conv)
+  ultimately
+  have "Atransform (ae, a) (\<Gamma>, Var x, S) \<Rightarrow>
+        ((x, Aeta_expand u (Aeta_expand_transform u e)) # map_ran (\<lambda>x e. Aeta_expand' (ae x) (Aeta_expand_transform' (ae x) e)) (delete x \<Gamma>), Aeta_expand u  (Aeta_expand_transform u e), S)"
+    using `ae x = up \<cdot> u` by (auto intro: step.intros simp add: map_ran_delete)
+  also
+  have "\<dots> \<Rightarrow>\<^sup>* Atransform (ae, u) ((x, e) # delete x \<Gamma>, e, S)"
+    using `ae x = up \<cdot> u` by simp (rule Aeta_expand_correct[OF `ae \` upds S \<subseteq> {up \<cdot> 0}` `Astack ae S \<sqsubseteq> u`])
+  finally
+  have "Atransform (ae, a) (\<Gamma>, Var x, S) \<Rightarrow>\<^sup>* Atransform (ae, u) ((x, e) # delete x \<Gamma>, e, S)".
+  }
+  ultimately show ?case by blast
+next
+case (var\<^sub>3 x \<Gamma> e S)
+  hence "ae x = up\<cdot>0" by auto
+
+  have "up\<cdot>(Astack ae S) \<sqsubseteq> ae x" using var\<^sub>3 by (auto simp add: join_below_iff)
+  then obtain u where "ae x = up \<cdot> u" and "Astack ae S \<sqsubseteq> u" by (cases "ae x") auto
+
+  have "Aexp e\<cdot>(Astack ae S) \<sqsubseteq> Aexp e\<cdot>0" by (rule monofun_cfun_arg) simp
+  also have "\<dots> \<sqsubseteq> ae" using `ae x = up \<cdot> 0` var\<^sub>3 by auto
+  finally have "Aexp e\<cdot>(Astack ae S) \<sqsubseteq> ae" by this simp
+  hence "AE_consistent ae ((x, e) # \<Gamma>, e, S)" using var\<^sub>3 `ae x = up \<cdot> 0`
+    by (fastforce intro!: AE_consistentI  simp add: join_below_iff split:if_splits)+
+  moreover
+  have "Astack ae (Upd x # S) \<sqsubseteq> a" using var\<^sub>3 by auto
+  with `ae x = up \<cdot> 0`
+  have "a = 0" by auto
+  
+  have "Astack ae S \<sqsubseteq> 0" by simp
+  ultimately
+  have "consistent (ae, 0) ((x, e) # \<Gamma>, e, S)" by auto
+  moreover
+  have "Atransform (ae, a) (\<Gamma>, e, Upd x # S) \<Rightarrow> Atransform (ae, 0) ((x, e) # \<Gamma>, e, S)"
+    using `ae x = up\<cdot>0` `a = 0` var\<^sub>3 by (fastforce intro!: step.intros)
+  ultimately show ?case by blast
+next
+  case (let\<^sub>1 \<Delta> \<Gamma> S e)
+
+  show ?case sorry
+qed
+
+
+  sublocale AbstractTransform step consistent Atransform
+    apply default
+    using foo
+    apply blast
+    done
+
+end
+end
+
